Let
$$
v = a - \frac{x^2}{2}.
$$
Then 
$$
v'(x) = -x.
$$
From page 32, we need to find $g_i^*$ such that 
$$
v(g_i^* + g_{-i}^*) + g_i^*\cdot v'(g_i^* + g_{-i}^*) - c = 0. \tag {2}
$$
Substituting $v$ and $v'$ into $\ref{2}$, we get
$$
a - \frac{(g_1 + \cdots + g_n)^2}{2} + g_i\cdot -(g_1+  \cdots + g_n) - c = 0
$$
Since 
$$
g_i = \frac{c - a + \frac{(g_1 + \cdots + g_n)^2}{2}}{-(g_1  +\cdots + g_n)},
$$
the value for $g_1, g_2, \cdots, g_n$ is the same, we have $g_1 = \cdots = g_n$.

Therefore
$$
\begin{aligned}
a -\frac{n^2g_1^2}{2} - ng_1^2 - c = 0 \\
-\frac{n^2g_1^2}{2} - ng_1^2  = c - a \\
\frac{n^2g_1^2}{2} + ng_1^2  = a - c \\
g_1^2\left(\frac{n^2}{2} + n\right)  = a - c \\
g_1 = \sqrt{\frac{a - c}{\frac{n^2}{2} + n}} \\
g_1 = \sqrt{\frac{a - c}{\frac{n^2}{2} + n}} \\
g_1 = \sqrt{\frac{2(a - c)}{n^2 + 2n}}
\end{aligned}
$$


